From $a \mid b$ we have:
\begin{align*}
a &\mid b  \\
\THEREFORE ax &= b \text{ for some integer $x$} & & \text{by ?} \tag{A}
\end{align*}
From $b \mid c$ we have:
\begin{align*}
b &\mid c  \\
\THEREFORE by &= c \text{ for some integer $y$} & & \text{by ?} \tag{B}
\end{align*}
From (A) and (B) (rewriting $b$ as $ax$ (A) in (B)) we have:
\begin{align*}
           (ax)y &= c \text{ for some integers $x, y$}                     \\
\THEREFORE a(xy) &= c \text{ for some integers $x, y$}     & & \text{by ?} \\
\THEREFORE a(xy) &= c \text{ for some integer  $xy$}       & & \text{by ?} \\
\THEREFORE az    &= c \text{ for some integers $z (= xy)$} & & \text{by ?} \\
\THEREFORE ? &\mid ?                                       & & \text{by ?} 
\end{align*}

