From $a \mid b$ we have:
\begin{align*}
a &\mid b  \\
\THEREFORE ax &= b \text{ for some integer $x$} & & \text{by ?} \tag{A}
\end{align*}
From $a \mid c$ we have:
\begin{align*}
a &\mid c  \\
\THEREFORE ay &= ? \text{ for some integer $?$} & & \text{by ?} \tag{B}
\end{align*}
From (A) and (B) we have:
\begin{align*}
           ax + ay &= b + ? \text{ for some integers $x, y$}               \\
\THEREFORE a?  &= b + ? \text{ for some integers $x, y$}     & & \text{by ?} \\
\THEREFORE a?  &= b + ? \text{ for some integer $x + y$}     & & \text{by ?} \\
\THEREFORE az  &= b + ? \text{ for some integers $z (= ?)$}  & & \text{by ?} \\
\THEREFORE ?   &\mid ?                                       & & \text{by ?} 
\end{align*}

